flush proof

disk-betree/ImplModelCache.i.dfy
@@ -1,8 +1,10 @@
 include "ImplModel.i.dfy"
+include "ImplModelIO.i.dfy"
 include "../lib/Sets.i.dfy"
 
 module ImplModelCache { 
   import opened ImplModel
+  import opened ImplModelIO
 
   import opened Options
   import opened Maps
@@ -16,11 +18,13 @@ module ImplModelCache {
     && s.Ready?
     && ref !in s.ephemeralIndirectionTable
     && ref !in s.cache 
+    && ref != BT.G.Root()
   }
 
   function getFreeRefIterate(s: Variables, i: uint64) 
   : (ref : Option<BT.G.Reference>)
   requires s.Ready?
+  requires i >= 1
   ensures ref.Some? ==> RefAvailable(s, ref.value)
   decreases 0x1_0000_0000_0000_0000 - i as int
   {
@@ -38,12 +42,13 @@ module ImplModelCache {
   requires s.Ready?
   ensures ref.Some? ==> RefAvailable(s, ref.value)
   {
-    getFreeRefIterate(s, 0)
+    getFreeRefIterate(s, 1)
   }
 
   function {:opaque} write(k: Constants, s: Variables, ref: BT.G.Reference, node: Node)
   : (s': Variables)
   requires s.Ready?
+  ensures s'.Ready?
   {
     // TODO how do we deal with this?
     var eph := s.ephemeralIndirectionTable[ref := (None, if node.children.Some? then node.children.value else [])];
@@ -53,6 +58,8 @@ module ImplModelCache {
   function {:opaque} alloc(k: Constants, s: Variables, node: Node)
   : (p: (Variables, Option<Reference>))
   requires s.Ready?
+  ensures var (s', id) := p;
+    s'.Ready?
   {
     var ref := getFreeRef(s);
     if ref.Some? then (
@@ -60,5 +67,39 @@ module ImplModelCache {
     ) else (
       (s, None)
     )
+  }
+ 
+  lemma allocCorrect(k: Constants, s: Variables, node: Node)
+  requires s.Ready?
+  requires WFVars(s)
+  requires WFNode(node)
+  requires BC.BlockPointsToValidReferences(INode(node), IIndirectionTable(s.ephemeralIndirectionTable).graph)
+  ensures var (s', ref) := alloc(k, s, node);
+    && WFVars(s')
+    && (ref.Some? ==> BC.Alloc(Ik(k), IVars(s), IVars(s'), ref.value, INode(node)))
+    && (ref.None? ==> s' == s)
+  {
+    reveal_alloc();
+    reveal_write();
+    var ref := getFreeRef(s);
+  }
+  
+  lemma writeCorrect(k: Constants, s: Variables, ref: BT.G.Reference, node: Node)
+  requires s.Ready?
+  requires WFVars(s)
+  requires ref in IIndirectionTable(s.ephemeralIndirectionTable).graph
+  requires ref in s.cache
+  requires ref == BT.G.Root() ==> s.rootBucket == map[]
+  requires WFNode(node)
+  requires BC.BlockPointsToValidReferences(INode(node), IIndirectionTable(s.ephemeralIndirectionTable).graph)
+  requires s.frozenIndirectionTable.Some? && ref in s.frozenIndirectionTable.value ==> s.frozenIndirectionTable.value[ref].0.Some?
+  ensures var s' := write(k, s, ref, node);
+    && WFVars(s')
+    && BC.Dirty(Ik(k), IVars(s), IVars(s'), ref, INode(node))
+  {
+    reveal_write();
+    if (ref == BT.G.Root()) {
+      INodeRootEqINodeForEmptyRootBucket(node);
+    }
   }
 }
