disk-betree/ImplModelFlush.i.dfy
@@ -1,8 +1,10 @@
 include "ImplModelCache.i.dfy"
+include "ImplModelIO.i.dfy"
 include "AsyncDiskModel.s.dfy"
 
 module ImplModelFlush { 
   import opened ImplModel
+  import opened ImplModelIO
   import opened ImplModelCache
 
   import opened Options
@@ -15,9 +17,21 @@ module ImplModelFlush {
   import opened NativeTypes
   import D = AsyncDisk
 
-  function flush(k: Constants, s: Variables, parentref: BT.G.Reference, slot: int)
-  : (Variables, DiskOp)
+  lemma lemmaChildInGraph(k: Constants, s: Variables, ref: BT.G.Reference, childref: BT.G.Reference)
+  requires s.Ready?
   requires Inv(k, s)
+  requires ref in s.cache
+  requires ref in s.ephemeralIndirectionTable
+  requires childref in BT.G.Successors(INode(s.cache[ref]))
+  ensures childref in s.ephemeralIndirectionTable
+  {
+    assert childref in IIndirectionTable(s.ephemeralIndirectionTable).graph[ref];
+  }
+
+  function flush(k: Constants, s: Variables, io: IO, parentref: BT.G.Reference, slot: int)
+  : (Variables, IO)
+  requires Inv(k, s)
+  requires io.IOInit?
   requires s.Ready?
   requires parentref in s.ephemeralIndirectionTable
   requires parentref in s.cache
@@ -32,11 +46,16 @@ module ImplModelFlush {
       && var (loc, _) := entry;
       && loc.None?
     ) then (
-      (s, D.NoDiskOp)
+      (s, io)
     ) else (
       var node := s.cache[parentref];
       var childref := node.children.value[slot];
+
+      lemmaChildInGraph(k, s, parentref, childref);
+
       if (childref !in s.cache) then (
+        assert childref in IIndirectionTable(s.ephemeralIndirectionTable).graph;
+        assert childref in IIndirectionTable(s.ephemeralIndirectionTable).locs;
         PageInReq(k, s, io, childref)
       ) else (
         var child := s.cache[childref];
@@ -45,13 +64,13 @@ module ImplModelFlush {
           && |child.buckets| < 0x1_0000_0000_0000_0000
           && (forall i | 0 <= i < |child.buckets| :: |child.buckets[i].keys| < 0x4000_0000_0000_0000)
         )) then (
-          (s, NoDiskOp)
+          (s, io)
         ) else (
-          var newbuckets := KMTable.Flush(node.buckets[slot], child.buckets, child.pivotTable);
+          var newbuckets := KMTable.flush(node.buckets[slot], child.buckets, child.pivotTable);
           var newchild := child.(buckets := newbuckets);
-          var s1, newchildref := alloc(k, s, newchild);
+          var (s1, newchildref) := alloc(k, s, newchild);
           if newchildref.None? then (
-            (s1, NoDiskOp)
+            (s1, io)
           ) else (
             var newparent := Node(
               node.pivotTable,
@@ -59,17 +78,97 @@ module ImplModelFlush {
               node.buckets[slot := KMTable.Empty()]
             );
             var s' := write(k, s1, parentref, newparent);
-            s'
+            (s', io)
           )
         )
       )
     )
   }
 
-  lemma flushCorrect(k: Constants, s: Variables, parentref: BT.G.Reference, slot: int)
-  requires flush.requires(k, s, parentref, slot)
+  lemma flushCorrect(k: Constants, s: Variables, io: IO, parentref: BT.G.Reference, slot: int)
+  requires flush.requires(k, s, io, parentref, slot)
   ensures
-      var (s', diskOp) := flush(k, s, parentref, slot);
+      var (s', io') := flush(k, s, io, parentref, slot);
       && WFVars(s')
-      && ImplADM.M.Next(Ik(k), I(k, s), I(k, s'), UI.NoOp, diskOp)
+      && M.Next(Ik(k), I(k, s), I(k, s'), UI.NoOp, diskOp(io'))
+  {
+    if (
+      && s.frozenIndirectionTable.Some?
+      && parentref in s.frozenIndirectionTable.value
+      && var entry := s.frozenIndirectionTable.value[parentref];
+      && var (loc, _) := entry;
+      && loc.None?
+    ) {
+      assert noop(k, IVars(s), IVars(s));
+    } else {
+      var node := s.cache[parentref];
+      var childref := node.children.value[slot];
+
+      lemmaChildInGraph(k, s, parentref, childref);
+      INodeRootEqINodeForEmptyRootBucket(node);
+
+      if (childref !in s.cache) {
+        assert childref in IIndirectionTable(s.ephemeralIndirectionTable).graph;
+        assert childref in IIndirectionTable(s.ephemeralIndirectionTable).locs;
+        PageInReqCorrect(k, s, io, childref);
+      } else {
+        var child := s.cache[childref];
+        INodeRootEqINodeForEmptyRootBucket(child);
+        if (!(
+          && |node.buckets[slot].keys| < 0x4000_0000_0000_0000
+          && |child.buckets| < 0x1_0000_0000_0000_0000
+          && (forall i | 0 <= i < |child.buckets| :: |child.buckets[i].keys| < 0x4000_0000_0000_0000)
+        )) {
+          assert noop(k, IVars(s), IVars(s));
+        } else {
+          var newbuckets := KMTable.flush(node.buckets[slot], child.buckets, child.pivotTable);
+          KMTable.flushRes(node.buckets[slot], child.buckets, child.pivotTable);
+          assume WFBuckets(newbuckets); // at the moment, only the KMTable.Flush method proves this.
+          WFBucketListFlush(KMTable.I(node.buckets[slot]), KMTable.ISeq(child.buckets), child.pivotTable);
+          
+          var newchild := child.(buckets := newbuckets);
+          var (s1, newchildref) := alloc(k, s, newchild);
+          reveal_alloc();
+          if newchildref.None? {
+            assert noop(k, IVars(s), IVars(s1));
+          } else {
+            var newparent := Node(
+              node.pivotTable,
+              Some(node.children.value[slot := newchildref.value]),
+              node.buckets[slot := KMTable.Empty()]
+            );
+            INodeRootEqINodeForEmptyRootBucket(newparent);
+
+            var s' := write(k, s1, parentref, newparent);
+            reveal_write();
+
+            forall ref | ref in BT.G.Successors(INode(newparent)) ensures ref in IIndirectionTable(s1.ephemeralIndirectionTable).graph {
+              if (ref == newchildref.value) {
+              } else {
+                assert ref in BT.G.Successors(INode(node));
+                lemmaChildInGraph(k, s, parentref, ref);
+                assert ref in IIndirectionTable(s1.ephemeralIndirectionTable).graph;
+              }
+            }
+            assert BC.BlockPointsToValidReferences(INode(newparent), IIndirectionTable(s1.ephemeralIndirectionTable).graph);
+
+            forall ref | ref in BT.G.Successors(INode(newchild)) ensures ref in IIndirectionTable(s.ephemeralIndirectionTable).graph {
+              lemmaChildInGraph(k, s, childref, ref);
+            }
+
+            allocCorrect(k, s, newchild);
+            writeCorrect(k, s1, parentref, newparent);
+
+            ghost var flushStep := BT.NodeFlush(parentref, INode(node), childref, INode(child), newchildref.value, INode(newchild), slot);
+            assert BT.ValidFlush(flushStep);
+            ghost var step := BT.BetreeFlush(flushStep);
+            assert INode(newparent) == BT.FlushOps(flushStep)[1].node;
+            assert BC.Dirty(Ik(k), IVars(s1), IVars(s'), parentref, INode(newparent));
+            BC.MakeTransaction2(Ik(k), IVars(s), IVars(s1), IVars(s'), BT.BetreeStepOps(step));
+            assert stepsBetree(k, IVars(s), IVars(s'), UI.NoOp, step);
+          }
+        }
+      }
+    }
+  }
 }
