disk-betree/ImplModelIO.i.dfy
@@ -1,7 +1,7 @@
 include "ImplModel.i.dfy"
 include "ByteBetreeBlockCache.i.dfy"
 
-module ImplIO { 
+module ImplModelIO { 
   import opened ImplModel
   import opened NativeTypes
   import opened Options
